src/Program.v
@@ -1,0 +1,51 @@
+Require Import Coq.Lists.List.
+
+Set Implicit Arguments.
+
+Inductive mem_op (N:Set) : Set :=
+| Read : N -> nat -> mem_op N
+| Write : N -> nat -> mem_op N.
+
+Inductive instruction N :=
+| Assign : N -> nat -> instruction N
+| Store : N -> N -> instruction N.
+
+Definition thread N := list (instruction N).
+
+Definition program N := list (thread N).
+
+Definition interp_thread_aux A N (prefixing : A -> mem_op N -> A) sum (i: instruction N) cont :=
+  match i with
+  | Assign x k => prefixing cont (Write x k)
+  | Store r x => sum (fun n => prefixing cont (Read x n)) end.
+
+Definition interp_thread A (N:Set) prefixing sum (empty : A) : thread N -> A :=
+  fold_right (interp_thread_aux prefixing sum) empty.
+
+Definition interp A (N:Set) parallel prefixing sum (empty : A) (p : program N) : A :=
+  parallel (fun i => nth i (map (interp_thread prefixing sum empty) p) empty).
+
+Require Import Causality.LTS.
+
+Definition interp_lts (N:Set) : program N -> LTS (mem_op N) :=
+  interp (@par_arbitrary_lts _ _)
+         (@prefixing_lts _) (@sum_arbitrary_lts _ _) (empty_lts _).
+
+Require Import Causality.ES.Definition.
+Require Import Causality.ES.Prefixing.
+Require Import Causality.ES.Parallel.
+Require Import Causality.ES.Sum.
+
+Require Import Coq.Logic.Eqdep_dec.
+Require Import Coq.Arith.PeanoNat.
+
+Module NatDecSet.
+  Definition U := nat.
+  Definition eq_dec : forall x y:U, {x = y} + {x <> y} := Nat.eq_dec.
+End NatDecSet.
+
+Module Par := ArbitraryParallel(NatDecSet).
+Module Sum := ArbitrarySum(NatDecSet).
+
+Definition interp_es (N:Set) : program N -> ES (mem_op N) :=
+  interp (@Par.par_arbitrary_es _) (@prefixing_es _) (@Sum.sum_arbitrary_es _) (empty_es _).
